\documentclass{article}

\title{Assignment Title}
\author{Your Name}
\date{\today}
\usepackage{amsmath} % for advanced math equations
\usepackage{amssymb} % for additional math symbols
\usepackage{amsfonts} % for math fonts
\usepackage{mathtools} % for additional math tools
\usepackage{amsthm} % for theorem environments
\usepackage[margin=1.5cm]{geometry}
\usepackage{enumitem}
\begin{document}

\maketitle

\section{CNF}
\begin{tabular}{ccccccccc}
    $P$ & $Q$  & $\neg Q$ & $P \lor Q$ & $P \land Q$ & $\neg Q \lor P$ & $\neg Q \land P$ & $Q \Rightarrow P$ & $P \iff Q$\\
    true&true&false&true&true&true&false&true&true\\
    true&false&true&true&false&true&true&true&false\\
    false&true&false&true&false&false&false&false&false\\
    false&false&true&false&false&true&false&true&true\\
\end{tabular}\\
so we can conclude that:
\begin{enumerate}
    \item $Q \Rightarrow P \equiv \neg Q \lor P$
    \item $Q \iff P \equiv P \Rightarrow Q \land P \Leftarrow Q $
    \item $P \iff Q \equiv Q \Rightarrow P \land P \Rightarrow Q  \equiv (\neg Q \lor P) \land (\neg P \lor Q)$
    \item $\neg \neg P \equiv P$
\end{enumerate}
convert each of the following formulas to CNF:
\subsection{1. $(P \Rightarrow \neg Q) \iff R$}
\begin{equation}
    Q \Rightarrow P \equiv \neg Q \lor P
\end{equation}
\subsection{2. $\neg (P \land \neg Q) \Rightarrow \neg R \lor \neg Q$}
\begin{equation}
    \begin{aligned}
        (P \Rightarrow \neg Q) \iff R &\overbrace{\equiv}^{\text{rule (2)}} (P \Rightarrow \neg Q) \Rightarrow R \land (P \Rightarrow \neg Q) \Leftarrow R\\
        &\overbrace{\equiv}^{\text{rule (1)}} (\neg (P \Rightarrow \neg Q) \lor R ) \land (( P \Rightarrow \neg Q) \lor \neg R)\\
        &\overbrace{\equiv}^{\text{rule (1)}} (\neg (\neg P \lor \neg Q) \lor R ) \land ((\neg P \lor \neg Q) \lor \neg R)\\
        &\overbrace{\equiv}^{\text{De Morgan}} ((  P \land  Q) \lor R) \land (\neg P \lor \neg Q \lor \neg R)\\
        &\overbrace{\equiv}^{\text{Distribution}} ( P \lor R) \land (  Q \lor R) \land  (\neg P \lor \neg Q \lor \neg R)
    \end{aligned}
\end{equation}
\subsection{3. $\neg (P \land  \neg Q) \Rightarrow (\neg R\lor \neg Q)$}
\begin{equation}
    \begin{aligned}
        \neg (P \land \neg Q) \Rightarrow \neg R \lor \neg Q &\overbrace{\equiv}^{\text{rule (1)}} (\neg(\neg(P \land \neg Q)) \lor (\neg R \lor \neg Q))\\
        &\overbrace{\equiv}^{\text{rule (4)}} ((P \land \neg Q) \lor \neg R \lor \neg Q)\\
        &\overbrace{\equiv}^{\text{Distribution}} (P \lor \neg R \lor \neg Q) \land (\neg Q \lor \neg R)
    \end{aligned}
\end{equation}
\subsection{4. $\neg (P \iff \neg Q) \Rightarrow R$}
\begin{equation}
    \begin{aligned}
        \neg (P \iff \neg Q) \Rightarrow R &\overbrace{\equiv}^{\text{rule (3)}} \neg ((\neg P \lor \neg Q) \land (Q \lor P)) \Rightarrow R\\
        &\overbrace{\equiv}^{\text{rule (1)}} \neg (\neg(( \neg P \lor \neg Q) \land  (Q \lor P))) \lor R\\
        &\overbrace{\equiv}^{\text{rule (4)}} (( \neg P \lor \neg Q) \land  (Q \lor P)) \lor R\\
        &\overbrace{\equiv}^{\text{Distribution}} (( \neg P \lor \neg Q) \lor R) \land ( (Q \lor P) \lor R)\\
        &\overbrace{\equiv}^{\text{}} ( \neg P \lor \neg Q \lor R) \land ( Q \lor P \lor R)\\
    \end{aligned}
\end{equation}
\subsection{5. $\neg (P \Rightarrow (\neg R \lor \neg Q)) \Rightarrow \neg R$}
\begin{equation}
    \begin{aligned}
        \neg (P \Rightarrow (\neg R \lor \neg Q)) \Rightarrow \neg R &\overbrace{\equiv}^{\text{rule (1)}} \neg (\neg P \lor \neg R \lor \neg Q) \Rightarrow \neg R\\
        &\overbrace{\equiv}^{\text{rule (1)}} \neg (\neg (\neg P \lor \neg R \lor \neg Q)) \lor \neg R\\
        &\overbrace{\equiv}^{\text{rule (4)}} \neg P \lor \neg R \lor \neg Q \lor \neg R\\
        &\overbrace{\equiv}^{\text{rule (4)}} \neg P \lor \neg R \lor \neg Q \lor \neg R\\
        &\overbrace{\equiv}^{\text{rule (4)}} \neg P \lor \neg R \lor \neg Q \lor \neg R
    \end{aligned}
\end{equation}


\section{Resolution}

\subsection{Given G = Nitay carries an umbrella}
Let's define the following predicates:
\begin{itemize}
    \item P = Nitay carries an umbrella
    \item R = If it rains
    \item W = Nitay dosen't get wet
\end{itemize}
So we can write the given statement as:
\begin{enumerate}
    \item $R \Rightarrow P \equiv \neg R \lor P$ 
    \item $P \Rightarrow W \equiv \neg P \lor W$
    \item $\neg R \Rightarrow W \equiv R \lor W$
    \item $ W$
    \item G = $P$
\end{enumerate}
Now we can start the algorithm, where KB=$(\neg R \lor P) \land (\neg P \lor W) \land (R \lor W) \land W$ and $\alpha =  P$\\
(for the sake of simplicity we will use the following notation: $Q \lor P = Q+P$ and $\neg Q = Q' $ and $Q \land P = QP$)
\begin{enumerate}
    \item we will define C = $KB \land \neg P$ 
    \item we will define new = $\emptyset$
    \item forall $C_i, C_j$ in C:
    \begin{enumerate}
        \item $(R'+P)(P'+W) = P'P+P'R' = P'R'$
        \item $(R'+P)(R+W) \equiv PR+PW+R'W$ 
        \item $(R'+P)(W) \equiv WR'+PW$ 
        \item $(R'+P)(P') \equiv P'R'+PP'\equiv R'P'$ 
        \item $(P'+W)(R+W) \equiv W+RP' $ 
        \item $(P'+W)(W) \equiv  P'W+W$ 
        \item $(P'+W)(P') \equiv P'+P'W $ 
        \item $(R+W)(W) \equiv RW+W $ 
        \item $(R+W)(P') \equiv P'R+WP'$ 
        \item $WP'$
    \end{enumerate}
    \item new = $\{P',R,(R'+P),(R+W),W,R',P',(P'+W)\}$
    \item new $\not\subset$ C
    \item C = C $\cup$ new
    \item forall $C_i, C_j$ in C:
    \begin{enumerate}
        \item $R'R \equiv \emptyset$
        \item since we got an empty clause will return true
    \end{enumerate}
\end{enumerate}
according to the algorithm, we can cann't conclude that the Nitay carries an umbrella.

\subsection{}
First we will define the following predicates:
\begin{itemize}
    \item $Z$: There is Noise
    \item $N$: Its night 
    \item $D$: Have dog 
    \item $C$: Have cat
    \item $M$: Have mice
    \item $P$: Struggling to fall asleep
    \item $A$: Amit 
\end{itemize}
So we can write the given statement as:
\begin{enumerate}
    \item All hounds (dogs) bark at night $\equiv (N \land D) \Rightarrow Z$
    \item If you have a cat, you don’t have mice $\equiv C \Rightarrow \neg M$
    \item If you have problems falling a sleep you don’t keep animals that make sound at night $\equiv P \Rightarrow \neg (N\land Z)$
    \item Amit has either a dog or a cat $\equiv A \Rightarrow (C\lor D)$
    \item G = If Amit have problems falling a sleep, then Amit has no mice $ \equiv \neg M \lor \neg A \lor \neg P $
\end{enumerate}
We would like to check if it is possible to conclude that if Amit has problems falling asleep, then Amit has no mice.\\
Let's start the algorithm, where KB=$\{\overline N + \overline D + Z,\overline C + M,\overline P + N+Z, \overline A + C+D\}$ and $\alpha = \overline M + \overline A + \overline P$\\

\begin{enumerate}
    \item we will define C = $KB \land \neg \alpha$
    \item we will define new = $\emptyset$
    \item forall $C_i, C_j$ in C:
    \begin{enumerate}
        \item $(\overline N + \overline D + Z)(\overline C + M)$ true when: $\overline N \cdot \overline C + \overline D\cdot \overline C + Z \overline C + \overline NM + \overline D M + ZM$
        \item $(\overline N + \overline D + Z)(\overline P + N + Z)$ true when: $\overline N \cdot \overline P +\overline N N + \overline N Z + \overline D \cdot \overline P + \overline D N + \overline D Z + Z \overline P + ZN + ZZ$
        \item $(\overline N + \overline D + Z)(\overline A + C + D)$ true when: $\overline N \cdot \overline A +\overline N C + \overline N D + \overline D  \cdot \overline A + \overline D C + \overline D D + Z \overline A + ZC + ZD$
        \item $(\overline N + \overline D + Z)( M)$ true when: $\overline{N}\cdot  {M} +\overline D \cdot   M + Z \cdot  M$
        \item $(\overline N + \overline D + Z)(A)$ true when: $\overline{N}\cdot  {A} +\overline D \cdot   A + Z \cdot  A$
        \item $(\overline N + \overline D + Z)(P)$ true when: $\overline{N}\cdot  {P} +\overline D \cdot   P + Z \cdot  P$
        \item $(\overline C + M)(\overline P + N + Z)$ true when: $\overline C \cdot \overline P + \overline C N + \overline C Z + M \overline P + M N +MZ$
        \item $(\overline C + M)(\overline A + C+D)$ true when: $\overline C \cdot \overline A + \overline C C + \overline C D + M \overline A + MC+MD$
        \item $(\overline C + M)(M)$ true when: $\overline C \cdot  M + MM$
        \item $(\overline C + M)(A)$ true when: $\overline C \cdot  A + MA$
        \item $(\overline C + M)(P)$ true when: $\overline C \cdot  P + MP$
        \item $(\overline P + N + Z)(\overline A + C + D)$ true when: $\overline P \cdot \overline A + \overline P C + \overline P D + N + \overline A + NC +ND + Z\overline A + Z C + Z D$
        \item $(\overline P + N + Z)(M)$ true when: $\overline P M + NM + ZM$
        \item $(\overline P + N + Z)(A)$ true when: $\overline P A + NA + ZA$
        \item $(\overline P + N + Z)(P)$ true when: $\overline P P + NP + ZP$
        \item $(\overline A + C + D)(M)$ true when: $\overline A M + C M + D M$
        \item $(\overline A + C + D)(A)$ true when: $\overline A A + C A + D A$
        \item $(\overline A + C + D)(P)$ true when: $\overline A P + C P + D P$
    \end{enumerate}
    \item new = $\{(\overline N + \overline D + Z), ( \overline C + M ),(\overline P + N + Z),(\overline A + C + D), M,A,P\}$
    \item we got that new $\subset$ C so we return false
    there is no condradiction between KB to "if Amit has problems falling asleep, then Amit has no mice".
\end{enumerate}
\end{document}